\aufgabe 2

\subsection*{Aufgabenteil a:}

$f(x) = \frac{1}{(1-x)^2}$\\
$f'(x) = \frac{2}{(1-x)^3}$\\
$f''(x) = \frac{6}{(1-x)^4}$\\
$f'''(x) = \frac{24}{(1-x)^5}$

\begin{align*}
P_0(x) =& \frac{1}{9} \\\\
P_1(x) =& \frac{1}{9} + \frac{2}{27}(x+2) \\
=& \frac{2}{27} x + \frac{3}{27} + \frac{4}{27}\\
=& \frac{2}{27} x + \frac{7}{27} \\\\
P_2(x) =& \frac{2}{27} x + \frac{7}{27} + \frac{1}{27} (x+2)^2 \\
=& \frac{2}{27} x + \frac{7}{27} + \frac{1}{27} x^2 \frac{4}{27} x + \frac{4}{27}\\
=& \frac{1}{27} x^2 + \frac{6}{27} x + \frac{11}{27} \\\\
P_3 =& \frac{1}{27} x^2 + \frac{6}{27} x + \frac{11}{27} + \frac{4}{243}(x+2)^3 \\
=& \frac{4}{243} x^3 + \frac{3}{81} x^2 + \frac{8}{81} x^2 + \frac{18}{81} x + \frac{16}{81} x + \frac{99}{243} + \frac{32}{243}\\
=& \frac{4}{243} x^3 + \frac{11}{81} x^2 + \frac{34}{81} x + \frac{131}{243}
\end{align*}

\subsubsection*{Intervalle:}
$g_0(x) = f(x) - P_0(x) = \frac{1}{(1-x)^2} - \frac{1}{9}$
$g_0(-4)=\frac{1}{25} - \frac{1}{9} = \frac{9}{225} - \frac{25}{225} = \frac{-16}{225}$\\
$g_0(0)=1 - \frac{1}{9} = \frac{8}{9}$\\
$I_0= P_0 + [-\frac{8}{9}, \frac{8}{9}]$\\\\

$g_1(x)=f(x) - P_1(x)= \frac{1}{(1-x)^2} - \frac{2}{27} x - \frac{7}{27}$\\
$g_1(-4) = \frac{1}{25} + \frac{8}{27} - \frac{7}{27} = \frac{1}{25} + \frac{1}{27}$ \\
$g_1(0) = 1 - \frac{7}{27} = \frac{20}{27}$\\
$I_1=P_1+[-\frac{20}{27},\frac{20}{27}]$\\\\

$g_2(x) =f(x) - P_2(x)= \frac{1}{(1-x)^2}-\frac{1}{27} x^2 - \frac{6}{27} x - \frac{11}{27}$\\
$g_2(-4)=\frac{1}{25}-\frac{16}{27}+\frac{24}{27}-\frac{11}{27}=\frac{1}{25}-\frac{3}{27}$\\
$g_2(0)=1-\frac{11}{27}=\frac{16}{27}$\\
$I_2=P_2+[-\frac{16}{27},\frac{16}{27}]$\\\\

$g_3(x) =f(x) - P_3(x)= \frac{1}{(1-x)^2}-\frac{4}{243} x^3 - \frac{11}{81} x^2 - \frac{34}{81} x - \frac{131}{243}$\\
$g_3(-4) = \frac{1}{25}+\frac{256}{243} - \frac{176}{81} + \frac{136}{81} - \frac{131}{243} =  \frac{1}{25} + \frac{125}{243} - \frac{40}{81} =  \frac{1}{25} + \frac{5}{243}$\\
$g_3(0)=1-\frac{131}{243} = \frac{112}{243}$\\
$I_3=P_3+[-\frac{112}{243},\frac{112}{243}]$
\subsection*{Aufgabenteil b:}
\begin{align*}
g_0=&x_0\\
g_1=&x_0+t+x_0t\\
g_2=&x_0+t+x_0t+t^2+x_0t^2\\
g_3=&x_0+t+x_0t+t^2+x_0t^2+t^3+x_0t^3\\
g_4=&g_3
\end{align*}
Fixpunkt erreicht.